\chapter{Tangent Spaces}
 
In this chapter we will generalize the notions that we covered in chapter 1 to manifolds.



\begin{definition}[Differential of a smooth map]
	Let $ F:N\to M $ be a smooth map between manifolds. This map induces a \emph{linear} map  called the \emph{differential of $ F $}
	\[ F_*: T_p N \to T_{F(p)}M \]
	where for $ X_P \in T_p N $ we have
	\[ (F_*(X_p))f = X_p(f\circ F) \]
	where $ f $ is a germ at $ p $.
\end{definition}

\begin{proposition}
	Let $ F:N\to M $. It differential $ F_* $ is a derivation at $ F(p) $ for $ p \in N $. 
\end{proposition}
\begin{proof}
	See \autoref{prob:DifferentialOfAMapIsADerivation}
\end{proof}





\section{Solved Problems}
\begin{problem}[The differential of a map]
	\label{prob:DifferentialOfAMapIsADerivation}
	Check that $ F_*(X_p) $ is a derivation at $ F(p) $ and that $ F_*: T_p N \to T_{F(p)}M  $ is a linear map.
\end{problem}
\begin{solution}
	We start with showing that $ F_*(X_p) $ is a derivation at $ F(p) $. By definition we have
	\begin{align*}
		[(F_*(X_p))(f\cdot g)](F(p)) &=  [ X_p((f\cdot g)\circ F) ](p) = [ X_p((f\circ F) \cdot (g\circ F)) ](p)\\
		&= [X_p(f\circ F)](p) \cdot g(F(p)) + f(F(p))\cdot [X_p(g\circ F)](p)\\
		&= [(F_*(X_p))f](F(p)) \cdot g(F(p)) + f(F(p))\cdot [(F_*(X_p))g].
 	\end{align*}
 	This shows that $ F_*(p) $ is indeed a derivation at $ F(p) $. Furthermore, to prove the linearity, let $ X_p, Y_p \in T_p(N) $. Then
 	\[ (F_*(X_p + Y_p))f = (X_p + Y_p)(f\circ F) = X_p(f\circ F) + Y_p(f\circ F) = (F_*(X_p)) f + (F_*(Y_p)) f. \]
\end{solution}